Java/src/Java/Func/Reify.v
@@ -1,5 +1,14 @@
 Require Import MirrorCore.Reify.Reify.
 Require Import MirrorCore.Lambda.Expr.
+Require Import MirrorCore.Views.ListView.
+Require Import MirrorCore.Views.ApplicativeView.
+Require Import MirrorCore.Views.ProdView.
+Require Import MirrorCore.Views.EqView.
+Require Import MirrorCore.Views.NatView.
+Require Import MirrorCore.Views.BoolView.
+Require Import MirrorCore.Views.StringView.
+Require Import MirrorCore.Views.ProdView.
+Require Import MirrorCore.Views.ListOpView.
 
 Require Import Java.Logic.AssertionLogic.
 Require Import Java.Logic.SpecLogic.
@@ -9,18 +18,16 @@ Require Import Java.Semantics.OperationalSemantics.
 Require Import Java.Func.JavaFunc.
 Require Import Java.Func.JavaType.
 
-Require Import Charge.ModularFunc.ILogicFunc.
-Require Import Charge.ModularFunc.BILogicFunc.
-Require Import Charge.ModularFunc.LaterFunc.
-Require Import Charge.ModularFunc.BaseFunc.
-Require Import Charge.ModularFunc.ListFunc.
-Require Import Charge.ModularFunc.OpenFunc.
-Require Import Charge.ModularFunc.EmbedFunc.
-Require Import Charge.Open.Stack.
-Require Import Charge.Open.Subst.
-Require Import Charge.Open.OpenILogic.
-Require Import Charge.Logics.BILogic.
-Require Import Charge.Logics.Later.
+Require Import Charge.Views.ILogicView.
+Require Import Charge.Views.BILogicView.
+Require Import Charge.Views.EmbedView.
+Require Import Charge.Views.SubstView.
+
+Require Import ChargeCore.Open.Stack.
+Require Import ChargeCore.Open.Subst.
+Require Import ChargeCore.Open.OpenILogic.
+Require Import ChargeCore.Logics.BILogic.
+Require Import ChargeCore.Logics.Later.
 
 Require Import ExtLib.Structures.Applicative.
 
@@ -36,8 +43,6 @@ Local Instance Applicative_Fun A : Applicative (Fun A) :=
 (*
 Reify Declare Patterns const_for_cmd += ((RHasType cmd ?0) => (fun (c : id cmd) => mkCmd [c] : expr typ func)).
 *)
-
-Require Import MirrorCore.Reify.Reify.
 
 Axiom t : Type.
 Reify Declare Patterns t_pat := t.
@@ -58,15 +63,15 @@ Reify Declare Typed Table term_table : BinNums.positive => reify_imp_typ.
 Require Import MirrorCore.ExprI.
 Require Import ExtLib.Data.SumN.
 
-Let Ext (x : SymEnv.func) := @ExprCore.Inj typ func (Into (ts := func_map) x 2 eq_refl).
+Let Ext (x : SymEnv.func) := @ExprCore.Inj typ func (Into (ts := func_map) 2 eq_refl x).
 
 Reify Declare Syntax reify_imp :=
   { (@Patterns.CFirst _
-  		((@Patterns.CVar _ (@ExprCore.Var typ func)) ::
-  	     (@Patterns.CPatterns _ patterns_java) ::
-         (@Patterns.CApp _ (@ExprCore.App typ func)) ::
-    	 (@Patterns.CAbs _ reify_imp_typ (@ExprCore.Abs typ func)) ::
-    	 (@Patterns.CTypedTable _ _ _ term_table Ext) :: nil))
+  		      ((@Patterns.CVar _ (@ExprCore.Var typ func)) ::
+                         (@Patterns.CPatterns _ patterns_java) ::
+                         (@Patterns.CApp _ (@ExprCore.App typ func)) ::
+    	                 (@Patterns.CAbs _ reify_imp_typ (@ExprCore.Abs typ func)) ::
+    	                 (@Patterns.CTypedTable _ _ _ term_table Ext) :: nil))
   }.
 
 Definition stack_get (x : Lang.var) (s : Lang.stack) := s x.
@@ -89,7 +94,6 @@ Definition set_fold_fun (x f : String.string) (P : sasn) :=
 *)
 Let _Inj := @ExprCore.Inj typ func.
 
-Require Import Java.Examples.ListModel.
 (*
 Reify Seed Typed Table term_table += 1 => [ (tyArr tyVal (tyArr (tyList tyVal) tyAsn)) , List ].
 Reify Seed Typed Table term_table += 2 => [ (tyArr tyVal (tyArr (tyList tyVal) tyAsn)) , NodeList ].
@@ -136,96 +140,96 @@ Reify Pattern patterns_java_typ += (!! @Subst.subst (String.string) val) => tySu
 Reify Pattern patterns_java_typ += (!! Fun @ ?0 @ ?1) => (fun (a b : function reify_imp_typ) => tyArr a b).
 
 Reify Pattern patterns_java += (RHasType String.string (?0)) => (fun (s : id String.string) => mkString (func := func) (typ := typ) s).
-Reify Pattern patterns_java += (RHasType field (?0)) => (fun (f : id field) => mkString (func := func) f).
-Reify Pattern patterns_java += (RHasType Lang.var (?0)) => (fun (f : id Lang.var) => mkString (func := func) f).
-Reify Pattern patterns_java += (RHasType val (?0)) => (fun (v : id val) => mkVal v).
-Reify Pattern patterns_java += (RHasType bool (?0)) => (fun (b : id bool) => mkBool (func := func) b).
-Reify Pattern patterns_java += (RHasType nat (?0)) => (fun (n : id nat) => mkNat (func := func) n).
-Reify Pattern patterns_java += (RHasType cmd (?0)) => (fun (c : id cmd) => mkCmd c).
-Reify Pattern patterns_java += (RHasType dexpr (?0)) => (fun (e : id dexpr) => mkDExpr e).
-Reify Pattern patterns_java += (RHasType Program (?0)) => (fun (P : id Program) => mkProg P).
-Reify Pattern patterns_java += (RHasType (list field) (?0)) => (fun (fs : id (list field)) => mkFields fs).
-Reify Pattern patterns_java += (RHasType class (?0)) => (fun (c : id class) => mkString (func := func) c).
+Reify Pattern patterns_java += (RHasType field (?0)) => (fun (f : id field) => mkString (typ := typ) (func := func) f).
+Reify Pattern patterns_java += (RHasType Lang.var (?0)) => (fun (f : id Lang.var) => mkString (typ := typ) (func := func) f).
+Reify Pattern patterns_java += (RHasType val (?0)) => (fun (v : id val) => Inj (typ := typ) (fVal v)).
+Reify Pattern patterns_java += (RHasType bool (?0)) => (fun (b : id bool) => mkBool (typ := typ) (func := func) b).
+Reify Pattern patterns_java += (RHasType nat (?0)) => (fun (n : id nat) => mkNat (typ := typ) (func := func) n).
+Reify Pattern patterns_java += (RHasType cmd (?0)) => (fun (c : id cmd) => Inj (typ := typ) (fCmd c)).
+Reify Pattern patterns_java += (RHasType dexpr (?0)) => (fun (e : id dexpr) => Inj (typ := typ) (fDExpr e)).
+Reify Pattern patterns_java += (RHasType Program (?0)) => (fun (P : id Program) => (Inj (typ := typ) (fProg P))).
+Reify Pattern patterns_java += (RHasType (list field) (?0)) => (fun (fs : id (list field)) => Inj (typ := typ) (fFields fs)).
+Reify Pattern patterns_java += (RHasType class (?0)) => (fun (c : id class) => mkString (typ := typ) (func := func) c).
 
 Reify Pattern patterns_java += (RHasType (@list dexpr) (?0)) => (fun (es : id (@list dexpr)) => mkExprList es).
-Reify Pattern patterns_java += (RHasType (@list String.string) (?0)) => (fun (vs : id (@list String.string)) => mkFields vs).
-Reify Pattern patterns_java += (!! (@eq) @ ?0) => (fun (x : function reify_imp_typ) => fEq (func := expr typ func) x).
+Reify Pattern patterns_java += (RHasType (@list String.string) (?0)) => (fun (vs : id (@list String.string)) => Inj (typ := typ) (fFields vs)).
+Reify Pattern patterns_java += (!! (@eq) @ ?0) => (fun (x : function reify_imp_typ) => Inj (typ := typ) (fEq (func := func) x)).
 
 (** Intuitionistic Operators **)
-Reify Pattern patterns_java += (!! @ILogic.lentails @ ?0 @ #) => (fun (x : function reify_imp_typ) => fEntails (func := expr typ func) x).
+Reify Pattern patterns_java += (!! @ILogic.lentails @ ?0 @ #) => (fun (x : function reify_imp_typ) => Inj (typ := typ) (fEntails x)).
 Reify Pattern patterns_java += (!! @ILogic.ltrue @ ?0 @ #) => (fun (x : function reify_imp_typ) => mkTrue (func := func) x).
 Reify Pattern patterns_java += (!! @ILogic.lfalse @ ?0 @ #) => (fun (x : function reify_imp_typ) => mkFalse (func := func) x).
 
-Reify Pattern patterns_java += (!! @ILogic.land @ ?0 @ #) => (fun (x : function reify_imp_typ) => fAnd (func := expr typ func) x).
-Reify Pattern patterns_java += (!! @ILogic.lor @ ?0 @ #) => (fun (x : function reify_imp_typ) => fOr (func := expr typ func) x).
-Reify Pattern patterns_java += (!! @ILogic.limpl @ ?0 @ #) => (fun (x : function reify_imp_typ) => fImpl (func := expr typ func) x).
+Reify Pattern patterns_java += (!! @ILogic.land @ ?0 @ #) => (fun (x : function reify_imp_typ) => Inj (typ := typ) (fAnd (func := func) x)).
+Reify Pattern patterns_java += (!! @ILogic.lor @ ?0 @ #) => (fun (x : function reify_imp_typ) => Inj (typ := typ) (fOr (func := func) x)).
+Reify Pattern patterns_java += (!! @ILogic.limpl @ ?0 @ #) => (fun (x : function reify_imp_typ) => Inj (typ := typ) (fImpl (func := func) x)).
 
-Reify Pattern patterns_java += (!! @ILogic.lexists @ ?0 @ # @ ?1) => (fun (x y : function reify_imp_typ) => fExists (func := expr typ func) y x).
+Reify Pattern patterns_java += (!! @ILogic.lexists @ ?0 @ # @ ?1) => (fun (x y : function reify_imp_typ) => Inj (typ := typ) (fExists (func := func) y x)).
 
-Reify Pattern patterns_java += (!! @ILogic.lforall @ ?0 @ # @ ?1) => (fun (x y : function reify_imp_typ) => fForall (func := expr typ func) y x).
+Reify Pattern patterns_java += (!! @ILogic.lforall @ ?0 @ # @ ?1) => (fun (x y : function reify_imp_typ) => Inj (typ := typ) (fForall (func := func) y x)).
 (** Embedding Operators **)
-Reify Pattern patterns_java += (!! @ILEmbed.embed @ ?0 @ ?1 @ #) => (fun (x y : function reify_imp_typ) => fEmbed (func := expr typ func) x y).
+Reify Pattern patterns_java += (!! @ILEmbed.embed @ ?0 @ ?1 @ #) => (fun (x y : function reify_imp_typ) => Inj (typ := typ) (fEmbed (func := func) x y)).
 
-Reify Pattern patterns_java += (!! @pair @ ?0 @ ?1) => (fun (x y : function reify_imp_typ) => fPair (func := expr typ func) x y).
+Reify Pattern patterns_java += (!! @pair @ ?0 @ ?1) => (fun (x y : function reify_imp_typ) => Inj (typ := typ) (fPair (func := func) x y)).
 
 (** Special cases for Coq's primitives **)
 Reify Pattern patterns_java += (!! True) => (mkTrue (func := func) tyProp).
 Reify Pattern patterns_java += (!! False) => (mkFalse (func := func) tyProp).
-Reify Pattern patterns_java += (!! and) => (fAnd (func := expr typ func) tyProp).
+Reify Pattern patterns_java += (!! and) => (Inj (typ := typ) (fAnd (func := func) tyProp)).
 
-Reify Pattern patterns_java += (!! or) => (fOr (func := expr typ func) tyProp).
+Reify Pattern patterns_java += (!! or) => (Inj (typ := typ) (fOr (func := func) tyProp)).
 
-Reify Pattern patterns_java += (!! ex @ ?0) => (fun (x : function reify_imp_typ) => fExists (func := expr typ func) x tyProp).
+Reify Pattern patterns_java += (!! ex @ ?0) => (fun (x : function reify_imp_typ) => Inj (typ := typ) (fExists (func := func) x tyProp)).
 
 Reify Pattern patterns_java += (RPi (?0) (?1)) => (fun (x : function reify_imp_typ) (y : function reify_imp) =>
-                                                   ExprCore.App (fForall (func := expr typ func) x tyProp) (ExprCore.Abs x y)).
+                                                   ExprCore.App (Inj (fForall (func := func) x tyProp)) (ExprCore.Abs x y)).
 
 Reify Pattern patterns_java += (RImpl (?0) (?1)) => (fun (x y : function reify_imp) => 
-	ExprCore.App (ExprCore.App (fImpl (func := expr typ func) tyProp) x) y).
+	ExprCore.App (ExprCore.App (Inj (fImpl (func := func) tyProp)) x) y).
 
 (** Separation Logic Operators **)
-Reify Pattern patterns_java += (!! @BILogic.sepSP @ ?0 @ #) => (fun (x : function reify_imp_typ) => (fStar (func := expr typ func) x)).
-Reify Pattern patterns_java += (!! @BILogic.wandSP @ ?0 @ #) => (fun (x : function reify_imp_typ) => (fWand (func := expr typ func) x)).
-Reify Pattern patterns_java += (!! @BILogic.empSP @ ?0 @ #) => (fun (x : function reify_imp_typ) => (mkEmp (func := func) x)).
-
-Reify Pattern patterns_java += (!! @Later.illater @ ?0 @ #) => (fun (x : function reify_imp_typ) => (fLater (func := expr typ func) x)).
-
+Reify Pattern patterns_java += (!! @BILogic.sepSP @ ?0 @ #) => (fun (x : function reify_imp_typ) => Inj (typ := typ) (fStar (func := func) x)).
+Reify Pattern patterns_java += (!! @BILogic.wandSP @ ?0 @ #) => (fun (x : function reify_imp_typ) => Inj (typ := typ) (fWand (func := func) x)).
+Reify Pattern patterns_java += (!! @BILogic.empSP @ ?0 @ #) => (fun (x : function reify_imp_typ) => Inj (typ := typ) (mkEmp (func := func) x)).
+(*
+Reify Pattern patterns_java += (!! @Later.illater @ ?0 @ #) => (fun (x : function reify_imp_typ) => (fLater (func := func) x)).
+*)
 Reify Pattern patterns_java += (!! method_spec) => (fMethodSpec).
 
 (** Program Logic **)
 
 
-Reify Pattern patterns_java += (!! triple) => (fTriple).
-Reify Pattern patterns_java += (!!method_lookup) => fMethodLookup.
-Reify Pattern patterns_java += (!!field_lookup) => fFieldLookup.
-Reify Pattern patterns_java += (!!m_ret) => fMethodRet.
-Reify Pattern patterns_java += (!!m_body) => fMethodBody.
-Reify Pattern patterns_java += (!!m_params) => fMethodArgs.
+Reify Pattern patterns_java += (!! triple) => (Inj (typ := typ) fTriple).
+Reify Pattern patterns_java += (!!method_lookup) => (Inj (typ := typ) fMethodLookup).
+Reify Pattern patterns_java += (!!field_lookup) => (Inj (typ := typ) fFieldLookup).
+Reify Pattern patterns_java += (!!m_ret) => (Inj (typ := typ) fMethodRet).
+Reify Pattern patterns_java += (!!m_body) => (Inj (typ := typ) fMethodBody).
+Reify Pattern patterns_java += (!!m_params) => (Inj (typ := typ) fMethodArgs).
 
 Reify Pattern patterns_java += (!! eval @ (RHasType dexpr (?0))) => (fun e : id dexpr => evalDExpr e).
-Reify Pattern patterns_java += (!! stack_get) => (fStackGet (typ := typ) (func := expr typ func)).
-Reify Pattern patterns_java += (!! stack_add (val := val)) => (fStackSet (typ := typ) (func := expr typ func)).
+Reify Pattern patterns_java += (!! stack_get) => (Inj (typ := typ) (fStackGet (typ := typ) (func := func))).
+Reify Pattern patterns_java += (!! stack_add (val := val)) => (Inj (typ := typ) (fStackSet (typ := typ) (func := func))).
 
-Reify Pattern patterns_java += (!! pointsto) => (fPointsto).
-Reify Pattern patterns_java += (!! prog_eq) => (fProgEq).
-Reify Pattern patterns_java += (!! typeof) => (fTypeOf).
+Reify Pattern patterns_java += (!! pointsto) => (Inj (typ := typ) fPointsto).
+Reify Pattern patterns_java += (!! prog_eq) => (Inj (typ := typ) fProgEq).
+Reify Pattern patterns_java += (!! typeof) => (Inj (typ := typ) fTypeOf).
 
-Reify Pattern patterns_java += (!! (@substl_trunc Lang.var val _)) => (fTruncSubst (func := expr typ func) (typ := typ)).
-Reify Pattern patterns_java += (!! (@substl Lang.var val _)) => (fSubst (func := expr typ func) (typ := typ)).
+Reify Pattern patterns_java += (!! (@substl_trunc Lang.var val _)) => (Inj (typ := typ) (fTruncSubst (func := func) (typ := typ))).
+Reify Pattern patterns_java += (!! (@substl Lang.var val _)) => (Inj (typ := typ) (fSubst (func := func) (typ := typ))).
 
-Reify Pattern patterns_java += (!! @nil @ ?0) => (fun (x : function reify_imp_typ) => (fNil (func := expr typ func) x)).
-Reify Pattern patterns_java += (!! @cons @ ?0) => (fun (x : function reify_imp_typ) => (fCons (func := expr typ func) x)).
-Reify Pattern patterns_java += (!! @length @ ?0) => (fun (x : function reify_imp_typ) => (fLength (func := expr typ func) x)).
-Reify Pattern patterns_java += (!! @zip @ ?0 @ ?1) => (fun (x y : function reify_imp_typ) => (fZip (func := expr typ func) x y)).
-Reify Pattern patterns_java += (!! @map @ ?0 @ ?1) => (fun (x y : function reify_imp_typ) => (fMap (func := expr typ func) x y)).
-Reify Pattern patterns_java += (!! @fold_right @ ?0 @ ?1) => (fun (x y : function reify_imp_typ) => (fFold (func := expr typ func) x y)).
+Reify Pattern patterns_java += (!! @nil @ ?0) => (fun (x : function reify_imp_typ) => (Inj (typ := typ) (fNil (func := func) x))).
+Reify Pattern patterns_java += (!! @cons @ ?0) => (fun (x : function reify_imp_typ) => (Inj (typ := typ) (fCons (func := func) x))).
+Reify Pattern patterns_java += (!! @length @ ?0) => (fun (x : function reify_imp_typ) => (Inj (typ := typ) (fLength (func := func) x))).
+Reify Pattern patterns_java += (!! @zip @ ?0 @ ?1) => (fun (x y : function reify_imp_typ) => (Inj (typ := typ) (fCombine (func := func) x y))).
+Reify Pattern patterns_java += (!! @map @ ?0 @ ?1) => (fun (x y : function reify_imp_typ) => (Inj (typ := typ) (fMap (func := func) x y))).
+Reify Pattern patterns_java += (!! @fold_right @ ?0 @ ?1) => (fun (x y : function reify_imp_typ) => (Inj (typ := typ) (fFold (func := func) x y))).
 
-Reify Pattern patterns_java += (!! (@apply_subst Lang.var val) @ ?0) => (fun (x : function reify_imp_typ) => fApplySubst (func := expr typ func) x).
-Reify Pattern patterns_java += (!! @subst1 Lang.var val _) => (fSingleSubst (func := expr typ func)).
-Reify Pattern patterns_java += (!! @field_lookup) => (fFieldLookup).
+Reify Pattern patterns_java += (!! (@apply_subst Lang.var val) @ ?0) => (fun (x : function reify_imp_typ) => Inj (typ := typ) (fApplySubst (func := func) x)).
+Reify Pattern patterns_java += (!! @subst1 Lang.var val _) => (Inj (typ := typ) (fSingleSubst (func := func))).
+Reify Pattern patterns_java += (!! @field_lookup) => (Inj (typ := typ) fFieldLookup).
 (** Applicative **)
-Reify Pattern patterns_java += (!! @Applicative.ap @ !! (Fun Lang.stack) @ # @ ?0 @ ?1) => (fun (x y : function reify_imp_typ) => fAp (func := expr typ func) x y).
-Reify Pattern patterns_java += (!! @Applicative.pure @ !! (Fun Lang.stack) @ # @ ?0) => (fun (x : function reify_imp_typ) => fConst (func := expr typ func) x).
+Reify Pattern patterns_java += (!! @Applicative.ap @ !! (Fun Lang.stack) @ # @ ?0 @ ?1) => (fun (x y : function reify_imp_typ) => Inj (typ := typ) (fAp (func := func) x y)).
+Reify Pattern patterns_java += (!! @Applicative.pure @ !! (Fun Lang.stack) @ # @ ?0) => (fun (x : function reify_imp_typ) => Inj (typ := typ) (fPure (func := func) x)).
 
 Let elem_ctor : forall x : typ, typD x -> @SymEnv.function _ _ :=
   @SymEnv.F _ _.
@@ -241,6 +245,7 @@ Require Import ILogic.
 
 Goal (forall (Pr : Program) (C : class) (v : val) (fields : list field), True).
   intros Pr C v fields.
+
   reify_imp (typeof C v).
 
   reify_imp (field_lookup).
@@ -264,8 +269,10 @@ Goal (forall (Pr : Program) (C : class) (v : val) (fields : list field), True).
   pose (E_val (vint 3)) as d.
 
   reify_imp ((ap (ap (T := Fun Lang.stack) (pure (@eq val)) (eval d)) (pure (vbool true)))).
-  
+
   generalize String.EmptyString. intro c.
+  reify_imp (cread c c c).
+
    reify_imp (ltrue |-- {[ ltrue ]} cread c c c {[ ltrue ]}).
 
   reify_imp cskip.
@@ -274,6 +281,7 @@ Goal (forall (Pr : Program) (C : class) (v : val) (fields : list field), True).
 
   reify_imp (forall x : nat, x = x).
   reify_imp (exists x : nat, x = x).
+
   reify_imp (@map nat nat).
   reify_imp (@subst1 Lang.var val _).
   reify_imp (cseq cskip cskip).
@@ -294,6 +302,7 @@ Goal (forall (Pr : Program) (C : class) (v : val) (fields : list field), True).
   reify_imp (x = x).
 
   reify_imp (@ltrue sasn _).
+
   exact I.
 
 Defined.
