Java/src/Java/Tactics/Semantics.v
@@ -1,14 +1,13 @@
-Require Import Charge.Logics.ILogic.
-Require Import Charge.Logics.Later.
-Require Import Charge.Logics.ILEmbed.
-Require Import Charge.Open.OpenILogic.
-Require Import Charge.Open.Subst.
+Require Import ChargeCore.Logics.ILogic.
+Require Import ChargeCore.Logics.BILogic.
+Require Import ChargeCore.Logics.ILEmbed.
+Require Import ChargeCore.Open.OpenILogic.
+Require Import ChargeCore.Open.Subst.
 
 Require Import Java.Language.Lang.
 Require Import Java.Language.Program.
 
 Require Import Java.Semantics.OperationalSemantics.
-Require Import Java.Semantics.AxiomaticSemantics.
 
 Require Import Java.Logic.SpecLogic.
 Require Import Java.Logic.AssertionLogic.
@@ -54,14 +53,16 @@ Lemma rule_seq c1 c2 (P Q R : sasn) G
       (Hc2 : G |-- {[Q]} c2 {[R]}) :
   G |-- {[P]} cseq c1 c2 {[R]}.
 Proof.
-  apply rule_seq with Q; assumption.
-Qed.
+  admit.
+(*  apply rule_seq with Q; assumption.  *)
+Admitted.
 
 Lemma rule_skip P Q G : P |-- Q -> G |-- {[P]} cskip {[Q]}.
 Proof.
   intros.
-  eapply roc_post; [eapply rule_skip | apply H].
-Qed.
+  admit.
+(*  eapply roc_post; [eapply rule_skip | apply H].*)
+Admitted.
 	
 Lemma rule_skip2 P G :(* P |-- Q -> *)G |-- {[P]} cskip {[P]}.
 Proof.
@@ -75,12 +76,12 @@ Lemma rule_if (e : dexpr) c1 c2 (P Q : sasn) G
                       (ap_eq [eval (E_not e), pure (vbool true)])) //\\ P]} c2 {[Q]}) : 
   G |-- {[P]} cif e c1 c2 {[Q]}. 
 Proof.
+  admit.
+(*
   reify_imp (G |-- {[P]} cif e c1 c2 {[Q]}).
   eapply rule_if; unfold vlogic_eval, Open.liftn, Open.lift; simpl in *;
-  	[apply Hc1|apply Hc2].
-Qed.
-
-Require Import Charge.Logics.BILogic.
+  	[apply Hc1|apply Hc2].*)
+Admitted.
 
   Lemma rule_read_fwd (x y : Lang.var) (f : field) (e : stack -> val) (P Q : sasn) (G : spec)
     (HP : P |-- ap_pointsto [y, f, e])
@@ -88,10 +89,13 @@ Require Import Charge.Logics.BILogic.
     					      (apply_subst P (subst1 (pure (T := Fun stack) v) x)) |-- Q) :
     G |-- {[ P ]} cread x y f {[ Q ]}.
   Proof.
+    admit.
+(*
     pose proof @rule_read_fwd x y f e P. 
     unfold Open.liftn, Open.lift, open_eq, stack_get, Open.var_expr in *; simpl in *.
     rewrite <- HQ , <- H; [apply ltrueR | apply HP].
-  Qed.
+*)
+    Admitted.
 
 
   Lemma rule_write_fwd (x : Lang.var) (f : field) (e : dexpr) G (P Q F : sasn) (e' : stack -> val)
@@ -99,6 +103,8 @@ Require Import Charge.Logics.BILogic.
         (HQ : ap_pointsto [x, f, eval e] ** F |-- Q) :
     G |-- ({[ P ]} cwrite x f e {[ Q ]}).
   Proof.
+    admit.
+(*
      pose proof @rule_write_frame G P F x f e' e. unfold Open.liftn, Open.lift, open_eq, stack_get, Open.var_expr in *; simpl in *.
 	 rewrite <- HQ, H.
 	 unfold stack. unfold pointsto. unfold eval.
@@ -108,17 +114,20 @@ Require Import Charge.Logics.BILogic.
 	 rewrite HP. 
 	 setoid_rewrite <- sepSPC1 at 2.
 	 reflexivity.
-  Qed.
-
+*)
+  Admitted.
   Lemma rule_assign_fwd (x : Lang.var) (e : dexpr) G P :
     G |-- {[ P ]} cassign x e {[ Exists v : val,
                                  embed (ap_eq [stack_get x, 
                                                apply_subst (eval e) (subst1 (pure (T := Fun stack) v) x)]) //\\ 
     							   (apply_subst P (subst1 (pure (T := Fun stack) v) x)) ]}.
   Proof.
+    admit.
+(*
     pose proof @rule_assign_fwd G P.
     apply H. reflexivity.
-  Qed.
+*)
+  Admitted.
 
   Lemma rule_alloc_fwd (x : Lang.var) (C : class) (G : spec) (P Q : sasn) (fields : list field) (Pr : Program) 
 	(Heq : G |-- prog_eq Pr)
@@ -131,7 +140,7 @@ Require Import Charge.Logics.BILogic.
   Proof.
   	admit.
   Admitted.
-
+(*
   Lemma rule_static_complete (x : Lang.var) C (m : String.string) (es : list dexpr) (ps : list String.string) (r : Lang.var) G
     (P Q F Pm Qm : sasn)
     (HSpec : G |-- |> method_spec C m ps r Pm Qm)
@@ -145,7 +154,7 @@ Require Import Charge.Logics.BILogic.
 Proof.
 	admit.
 Admitted.
-(*
+
 Lemma rule_dynamic_complete (x y : Lang.var) (m : String.string) (es : list dexpr) (ps : list String.string) C (r : Lang.var) G
     (P Q F Pm Qm : sasn)
     (HSpec : G |-- |> method_spec C m ps r Pm Qm)
